Fix compilation. Move VInt instances.

src/coq/Semantics/VellvmIntegers.v
@@ -62,73 +62,457 @@ Class VMemInt I : Type :=
     mdtyp_of_int : dtyp
   }.
 
-  Definition mequ_Z (x y : Z) : bool :=
-    Z.eqb x y.
+Definition mequ_Z (x y : Z) : bool :=
+  Z.eqb x y.
 
-  Definition mcmp_Z (c : Numeric.Integers.comparison) (x y : Z) : bool :=
-    match c with
-    | Ceq => Z.eqb x y
-    | Cne => Zneq_bool x y
-    | Clt => Z.ltb x y
-    | Cle => Z.leb x y
-    | Cgt => Z.gtb x y
-    | Cge => Z.geb x y
-    end.
+Definition mcmp_Z (c : Numeric.Integers.comparison) (x y : Z) : bool :=
+  match c with
+  | Ceq => Z.eqb x y
+  | Cne => Zneq_bool x y
+  | Clt => Z.ltb x y
+  | Cle => Z.leb x y
+  | Cgt => Z.gtb x y
+  | Cge => Z.geb x y
+  end.
 
-  Definition mcmpu_Z (c : Numeric.Integers.comparison) (x y : Z) : bool :=
-    match c with
-    | Ceq => Z.eqb x y
-    | Cne => Zneq_bool x y
-    | Clt => Z.ltb x y
-    | Cle => Z.leb x y
-    | Cgt => Z.gtb x y
-    | Cge => Z.geb x y
-    end.
+Definition mcmpu_Z (c : Numeric.Integers.comparison) (x y : Z) : bool :=
+  match c with
+  | Ceq => Z.eqb x y
+  | Cne => Zneq_bool x y
+  | Clt => Z.ltb x y
+  | Cle => Z.leb x y
+  | Cgt => Z.gtb x y
+  | Cge => Z.geb x y
+  end.
 
-  #[global] Instance VMemInt_Z : VMemInt Z :=
-    { mequ  := Z.eqb;
-      mcmp  := mcmp_Z;
-      mcmpu := mcmpu_Z;
+#[global] Instance VMemInt_Z : VMemInt Z :=
+  { mequ  := Z.eqb;
+    mcmp  := mcmp_Z;
+    mcmpu := mcmpu_Z;
 
-      mbitwidth := None;
-      mzero     := 0%Z;
-      mone      := 1%Z;
+    mbitwidth := None;
+    mzero     := 0%Z;
+    mone      := 1%Z;
 
-      madd := fun x y => ret (Z.add x y);
-      (* No overflows *)
-      madd_carry := fun x y c => 0%Z;
-      madd_overflow := fun x y c => 0%Z;
+    madd := fun x y => ret (Z.add x y);
+    (* No overflows *)
+    madd_carry := fun x y c => 0%Z;
+    madd_overflow := fun x y c => 0%Z;
 
-      msub := fun x y => ret (Z.sub x y);
-      (* No overflows *)
-      msub_borrow := fun x y c => 0%Z;
-      msub_overflow := fun x y c => 0%Z;
+    msub := fun x y => ret (Z.sub x y);
+    (* No overflows *)
+    msub_borrow := fun x y c => 0%Z;
+    msub_overflow := fun x y c => 0%Z;
 
-      mmul := fun x y => ret (Z.mul x y);
+    mmul := fun x y => ret (Z.mul x y);
 
-      mdivu := fun x y => Z.div x y;
-      mdivs := fun x y => ret (Z.div x y);
+    mdivu := fun x y => Z.div x y;
+    mdivs := fun x y => ret (Z.div x y);
 
-      mmodu := fun x y => Z.modulo x y;
-      mmods := fun x y => ret (Z.modulo x y);
+    mmodu := fun x y => Z.modulo x y;
+    mmods := fun x y => ret (Z.modulo x y);
 
-      mshl := fun x y => ret (Z.shiftl x y);
-      mshr := fun x y => Z.shiftr x y;
-      mshru := fun x y => Z.shiftr x y;
+    mshl := fun x y => ret (Z.shiftl x y);
+    mshr := fun x y => Z.shiftr x y;
+    mshru := fun x y => Z.shiftr x y;
 
-      mnegative := fun x => ret (0 - x)%Z;
+    mnegative := fun x => ret (0 - x)%Z;
 
-      mand := Z.land;
-      mor := Z.lor;
-      mxor := Z.lxor;
+    mand := Z.land;
+    mor := Z.lor;
+    mxor := Z.lxor;
 
-      mmin_signed := None;
-      mmax_signed := None;
+    mmin_signed := None;
+    mmax_signed := None;
 
-      munsigned := fun x => x;
-      msigned := fun x => x;
+    munsigned := fun x => x;
+    msigned := fun x => x;
 
-      mrepr := fun x => ret x;
+    mrepr := fun x => ret x;
 
-      mdtyp_of_int := DTYPE_IPTR
-    }.
+    mdtyp_of_int := DTYPE_IPTR
+  }.
+
+(* Set up representations for for i1, i32, and i64 *)
+Module Wordsize1.
+  Definition wordsize := 1%nat.
+  Remark wordsize_not_zero: wordsize <> 0%nat.
+  Proof using. unfold wordsize; congruence. Qed.
+End Wordsize1.
+
+Module Wordsize8.
+  Definition wordsize := 8%nat.
+  Remark wordsize_not_zero: wordsize <> 0%nat.
+  Proof using. unfold wordsize; congruence. Qed.
+End Wordsize8.
+
+Module Int1 := Make(Wordsize1).
+Module Int8 := Make(Wordsize8).
+Module Int16 := Integers.Int16.
+Module Int32 := Integers.Int.
+Module Int64 := Integers.Int64.
+
+Definition int1 := Int1.int.
+Definition int8 := Int8.int.
+Definition int16 := Int16.int.
+Definition int32 := Int32.int.
+Definition int64 := Int64.int.
+
+Class VInt I : Type :=
+  {
+    (* Comparisons *)
+    equ : I -> I -> bool;
+    cmp : comparison -> I -> I -> bool;
+    cmpu : comparison -> I -> I -> bool;
+
+    (* Constants *)
+    bitwidth : nat;
+    zero : I;
+    one : I;
+
+    (* Arithmetic *)
+    add : I -> I -> I;
+    add_carry : I -> I -> I -> I;
+    add_overflow : I -> I -> I -> I;
+
+    sub : I -> I -> I;
+    sub_borrow : I -> I -> I -> I;
+    sub_overflow : I -> I -> I -> I;
+
+    mul : I -> I -> I;
+
+    divu : I -> I -> I;
+    divs : I -> I -> I;
+    modu : I -> I -> I;
+    mods : I -> I -> I;
+
+    shl : I -> I -> I;
+    shr : I -> I -> I;
+    shru : I -> I -> I;
+
+    negative : I -> I;
+
+    (* Logic *)
+    and : I -> I -> I;
+    or : I -> I -> I;
+    xor : I -> I -> I;
+
+    (* Bounds *)
+    min_signed : Z;
+    max_signed : Z;
+
+    (* Conversion *)
+    unsigned : I -> Z;
+    signed : I -> Z;
+
+    repr : Z -> I;
+  }.
+
+#[global] Instance VInt32 : VInt Int32.int :=
+  {
+    (* Comparisons *)
+    equ := Int32.eq;
+    cmp := Int32.cmp;
+    cmpu := Int32.cmpu;
+
+    bitwidth := 32;
+
+    (* Constants *)
+    zero := Int32.zero;
+    one := Int32.one;
+
+    (* Arithmetic *)
+    add := Int32.add;
+    add_carry := Int32.add_carry;
+    add_overflow := Int32.add_overflow;
+
+    sub := Int32.sub;
+    sub_borrow := Int32.sub_borrow;
+    sub_overflow := Int32.sub_overflow;
+
+    mul := Int32.mul;
+
+    divu := Int32.divu;
+    divs := Int32.divs;
+    modu := Int32.modu;
+    mods := Int32.mods;
+
+    shl := Int32.shl;
+    shr := Int32.shr;
+    shru := Int32.shru;
+
+    negative := Int32.negative;
+
+    (* Logic *)
+    and := Int32.and;
+    or := Int32.or;
+    xor := Int32.xor;
+
+    (* Bounds *)
+    min_signed := Int32.min_signed;
+    max_signed := Int32.max_signed;
+
+    (* Conversion *)
+    unsigned := Int32.unsigned;
+    signed := Int32.signed;
+
+    repr := Int32.repr;
+  }.
+
+#[global] Instance VInt1 : VInt Int1.int :=
+  {
+    (* Comparisons *)
+    equ := Int1.eq;
+    cmp := Int1.cmp;
+    cmpu := Int1.cmpu;
+
+    bitwidth := 1;
+
+    (* Constants *)
+    zero := Int1.zero;
+    one := Int1.one;
+
+    (* Arithmetic *)
+    add := Int1.add;
+    add_carry := Int1.add_carry;
+    add_overflow := Int1.add_overflow;
+
+    sub := Int1.sub;
+    sub_borrow := Int1.sub_borrow;
+    sub_overflow := Int1.sub_overflow;
+
+    mul := Int1.mul;
+
+    divu := Int1.divu;
+    divs := Int1.divs;
+    modu := Int1.modu;
+    mods := Int1.mods;
+
+    shl := Int1.shl;
+    shr := Int1.shr;
+    shru := Int1.shru;
+
+    negative := Int1.negative;
+
+    (* Logic *)
+    and := Int1.and;
+    or := Int1.or;
+    xor := Int1.xor;
+
+    (* Bounds *)
+    min_signed := Int1.min_signed;
+    max_signed := Int1.max_signed;
+
+    (* Conversion *)
+    unsigned := Int1.unsigned;
+    signed := Int1.signed;
+
+    repr := Int1.repr;
+  }.
+
+#[global] Instance VInt8 : VInt Int8.int :=
+  {
+    (* Comparisons *)
+    equ := Int8.eq;
+    cmp := Int8.cmp;
+    cmpu := Int8.cmpu;
+
+    bitwidth := 8;
+
+    (* Constants *)
+    zero := Int8.zero;
+    one := Int8.one;
+
+    (* Arithmetic *)
+    add := Int8.add;
+    add_carry := Int8.add_carry;
+    add_overflow := Int8.add_overflow;
+
+    sub := Int8.sub;
+    sub_borrow := Int8.sub_borrow;
+    sub_overflow := Int8.sub_overflow;
+
+    mul := Int8.mul;
+
+    divu := Int8.divu;
+    divs := Int8.divs;
+    modu := Int8.modu;
+    mods := Int8.mods;
+
+    shl := Int8.shl;
+    shr := Int8.shr;
+    shru := Int8.shru;
+
+    negative := Int8.negative;
+
+    (* Logic *)
+    and := Int8.and;
+    or := Int8.or;
+    xor := Int8.xor;
+
+    (* Bounds *)
+    min_signed := Int8.min_signed;
+    max_signed := Int8.max_signed;
+
+    (* Conversion *)
+    unsigned := Int8.unsigned;
+    signed := Int8.signed;
+
+    repr := Int8.repr;
+  }.
+
+#[global] Instance VInt16 : VInt Int16.int :=
+  {
+    (* Comparisons *)
+    equ := Int16.eq;
+    cmp := Int16.cmp;
+    cmpu := Int16.cmpu;
+
+    bitwidth := 16;
+
+    (* Constants *)
+    zero := Int16.zero;
+    one := Int16.one;
+
+    (* Arithmetic *)
+    add := Int16.add;
+    add_carry := Int16.add_carry;
+    add_overflow := Int16.add_overflow;
+
+    sub := Int16.sub;
+    sub_borrow := Int16.sub_borrow;
+    sub_overflow := Int16.sub_overflow;
+
+    mul := Int16.mul;
+
+    divu := Int16.divu;
+    divs := Int16.divs;
+    modu := Int16.modu;
+    mods := Int16.mods;
+
+    shl := Int16.shl;
+    shr := Int16.shr;
+    shru := Int16.shru;
+
+    negative := Int16.negative;
+
+    (* Logic *)
+    and := Int16.and;
+    or := Int16.or;
+    xor := Int16.xor;
+
+    (* Bounds *)
+    min_signed := Int16.min_signed;
+    max_signed := Int16.max_signed;
+
+    (* Conversion *)
+    unsigned := Int16.unsigned;
+    signed := Int16.signed;
+
+    repr := Int16.repr;
+  }.
+
+#[global] Instance VIntVMemInt {I} `{VInt I} : VMemInt I :=
+  {
+    (* Comparisons *)
+    mequ := equ;
+    mcmp := cmp;
+    mcmpu := cmpu;
+
+    (* Constants *)
+    mbitwidth := ret bitwidth;
+    mzero := zero;
+    mone := one;
+
+    (* Arithmetic *)
+    madd := fun x y => ret (add x y);
+    madd_carry := add_carry;
+    madd_overflow := add_overflow;
+
+    msub := fun x y => ret (sub x y);
+    msub_borrow := sub_borrow;
+    msub_overflow := sub_overflow;
+
+    mmul := fun x y => ret (mul x y);
+
+    mdivu := divu;
+    mdivs := fun x y => ret (divs x y);
+
+    mmodu := modu;
+    mmods := fun x y => ret (mods x y);
+
+    mshl := fun x y => ret (shl x y);
+    mshr := shr;
+    mshru := shru;
+
+    mnegative := fun x => ret (negative x);
+
+    (* Logic *)
+    mand := and;
+    mor := or;
+    mxor := xor;
+
+    (* Bounds, possibly unbounded *)
+    mmin_signed := ret (min_signed);
+    mmax_signed := ret (max_signed);
+
+    (* Conversion *)
+    munsigned := unsigned;
+    msigned := signed;
+
+    mrepr := fun x => NoOom (repr x);
+
+    (* dtyp *)
+    mdtyp_of_int := DTYPE_I (N.of_nat bitwidth)
+  }.
+
+#[global] Instance VInt64 : VInt Int64.int :=
+  {
+    (* Comparisons *)
+    equ := Int64.eq;
+    cmp := Int64.cmp;
+    cmpu := Int64.cmpu;
+
+    bitwidth := 64;
+
+    (* Constants *)
+    zero := Int64.zero;
+    one := Int64.one;
+
+    (* Arithmetic *)
+    add := Int64.add;
+    add_carry := Int64.add_carry;
+    add_overflow := Int64.add_overflow;
+
+    sub := Int64.sub;
+    sub_borrow := Int64.sub_borrow;
+    sub_overflow := Int64.sub_overflow;
+
+    mul := Int64.mul;
+
+    divu := Int64.divu;
+    divs := Int64.divs;
+    modu := Int64.modu;
+    mods := Int64.mods;
+
+    shl := Int64.shl;
+    shr := Int64.shr;
+    shru := Int64.shru;
+
+    negative := Int64.negative;
+
+    (* Logic *)
+    and := Int64.and;
+    or := Int64.or;
+    xor := Int64.xor;
+
+    (* Bounds *)
+    min_signed := Int64.min_signed;
+    max_signed := Int64.max_signed;
+
+    (* Conversion *)
+    unsigned := Int64.unsigned;
+    signed := Int64.signed;
+
+    repr := Int64.repr;
+  }.
